finish Temporal_new.v, tweaks/progress in Typing_new.v

src/Temporal_new.v
@@ -34,7 +34,10 @@ From Paco Require Import
      paco.
 
 Import ITreeNotations.
+Import SumNotations.
+Open Scope sum_scope.
 
+Hint Constructors stepsF stepF : core.
 Hint Resolve no_errors_gen_mon : paco.
 Hint Resolve sbuter_gen_mon : paco.
 
@@ -49,7 +52,7 @@ Definition eq_sat_sep_sbuter {S1 S2 R1 R2} (q:@perm (S1*S2))
   forall p Q t1 s1 t2 s2, pre q (s1,s2) -> p ⊥ q ->
     sbuter p Q t1 s1 t2 s2 -> no_errors t2 s2 ->
     (P1 t1 s1 <-> P2 t2 s2).
-Hint Unfold eq_sat_sep_sbuter.
+Hint Unfold eq_sat_sep_sbuter : core.
 
 
 (** * `eq_sat_sep_sbuter` for state predicates **)
@@ -226,4 +229,231 @@ Proof.
         -- destruct H11; [|inversion H11]; eauto.
         -- eapply step_no_errors; eauto.
         -- specialize (H9 _ _ x); pclearbot; eauto.
+Qed.
+
+
+(** * `eq_sat_sep_sbuter` for `AU` **)
+
+Inductive AU {S R} (P P' : TPred S R) t0 s0 : Prop :=
+| AU_here : P' t0 s0 -> AU P P' t0 s0
+| AU_step : P t0 s0 -> steps t0 s0 ->
+            (forall t1 s1, step t0 s0 t1 s1 -> AU P P' t1 s1) ->
+            AU P P' t0 s0.
+
+Lemma eq_sat_AU {S1 S2 R1 R2} q (P1 P1' : TPred S1 R1) (P2 P2' : TPred S2 R2) :
+    eq_sat_sep_sbuter q P1 P2 -> eq_sat_sep_sbuter q P1' P2' ->
+    eq_sat_sep_sbuter q (AU P1 P1') (AU P2 P2').
+Proof.
+  intros eq_sat_Ps eq_sat_P's; split; intros.
+  - revert p t2 s2 H H0 H1 H2; dependent induction H3; intros.
+    { apply AU_here; eapply eq_sat_P's; eauto. }
+    punfold H5; red in H5; dependent induction H5.
+    + red in H0; destruct x0; inv H0.
+    + punfold H6; red in H6; destruct x; inv H6.
+    + destruct (stepsF_impl_stepF _ _ H0) as [?t1' [?s1' []]].
+      eapply (H2 _ _ X p'); eauto.
+      * respects; eapply sep_r; eauto.
+      * pfold; red; eapply H9; eauto.
+    + apply AU_step; eauto; intros.
+      * eapply eq_sat_Ps; eauto.
+        pfold; red; econstructor 4; eauto.
+      * eapply H10; eauto.
+        -- respects; eapply sep_r; eauto.
+        -- eapply step_no_errors; eauto.
+    + apply AU_step; eauto; intros.
+      * eapply eq_sat_Ps; eauto.
+        pfold; red; econstructor 5; eauto.
+      * specialize (H10 _ _ X); destruct H10 as [?t1' [?s1' [? []]]].
+        change (step t0 s1 t1' s1') in x.
+        eapply (H2 _ _ x p'); pclearbot; eauto.
+        -- respects; eapply sep_r; eauto.
+        -- eapply step_no_errors; eauto.
+  - revert p t1 s1 H H0 H1 H2; dependent induction H3; intros.
+    { apply AU_here; eapply eq_sat_P's; eauto. }
+    punfold H5; red in H5; dependent induction H5.
+    + red in H0; destruct x; inv H0.
+    + punfold H6; red in H6; destruct x; inv H6.
+    + apply AU_step; eauto; intros.
+      * eapply eq_sat_Ps; eauto.
+        pfold; red; econstructor 3; eauto.
+      * eapply H10; eauto.
+        respects; eapply sep_r; eauto.
+    + destruct (stepsF_impl_stepF _ _ H0) as [?t2' [?s2' []]].
+      eapply (H2 _ _ X p'); eauto.
+      * respects; eapply sep_r; eauto.
+      * pfold; red; eapply H9; eauto.
+      * eapply step_no_errors; eauto.
+    + apply AU_step; eauto; intros.
+      * eapply eq_sat_Ps; eauto.
+        pfold; red; econstructor 5; eauto.
+      * specialize (H9 _ _ X); destruct H9 as [?t2' [?s2' [? []]]].
+        change (step t0 s2 t2' s2') in x.
+        eapply (H2 _ _ x p'); pclearbot; eauto.
+        -- respects; eapply sep_r; eauto.
+        -- eapply step_no_errors; eauto.
+Qed.
+
+
+(** * `eq_sat_sep_sbuter` for `AF` **)
+
+Definition AF {S R} := @AU S R (fun _ _ => True).
+
+Lemma eq_sat_AF {S1 S2 R1 R2} q (P1 : TPred S1 R1) (P2 : TPred S2 R2) :
+    eq_sat_sep_sbuter q P1 P2 ->
+    eq_sat_sep_sbuter q (AF P1) (AF P2).
+Proof. apply eq_sat_AU; easy. Qed.
+
+
+(** * `eq_sat_sep_sbuter` for `EG` **)
+
+Inductive EG_gen {S R} (P : TPred S R) EG t0 s0 : Prop :=
+| EG_step t1 s1 : P t0 s0 -> step t0 s0 t1 s1 -> EG t1 s1 -> EG_gen P EG t0 s0
+| EG_stop : P t0 s0 -> ~ (steps t0 s0) -> EG_gen P EG t0 s0.
+Arguments EG_step {S R P EG t0 s0} t1 s1.
+Arguments EG_stop {S R P EG t0 s0}.
+
+Definition EG {S R} P := paco2 (@EG_gen S R P) bot2.
+
+Lemma EG_gen_mon {S R P} : monotone2 (@EG_gen S R P).
+Proof. repeat intro; induction IN; subst; solve [econstructor; eauto]. Qed.
+Hint Resolve EG_gen_mon : paco.
+
+Definition EG_pf {S R P t0 s0} : @EG S R P t0 s0 -> P t0 s0.
+Proof. intro; punfold H; destruct H; eauto. Defined.
+
+Lemma eq_sat_EG {S1 S2 R1 R2} q (P1 : TPred S1 R1) (P2 : TPred S2 R2) :
+    eq_sat_sep_sbuter q P1 P2 ->
+    eq_sat_sep_sbuter q (EG P1) (EG P2).
+Proof.
+  intro eq_sat_Ps; split; intros.
+  - revert p t1 s1 t2 s2 H H0 H1 H2 H3; pcofix CIH; intros.
+    punfold H2; red in H2; dependent induction H2.
+    + pfold; apply EG_stop.
+      * apply EG_pf in H2.
+        eapply eq_sat_Ps; eauto.
+        pfold; red; econstructor 1; eauto.
+      * intro; red in H6; destruct x; inv H6.
+    + punfold H3; red in H3; destruct x; inv H3.
+    + punfold H8; destruct H8; [| exfalso; apply H9; red; eauto ].
+      eapply H4; pclearbot; eauto.
+      respects; eapply sep_r; eauto.
+    + destruct (stepsF_impl_stepF _ _ H6) as [?t2' [?s2' []]].
+      change (step t2 s2 t2' s2') in X.
+      pfold; apply (EG_step t2' s2'); eauto.
+      * apply EG_pf in H8.
+        eapply eq_sat_Ps; eauto.
+        pfold; econstructor 4; eauto.
+      * left; eapply H4; eauto.
+        -- respects; eapply sep_r; eauto.
+        -- eapply step_no_errors; eauto.
+    + punfold H8; destruct H8; [| exfalso; apply H9; red; eauto ].
+      destruct (H3 _ _ X) as [?t2' [?s2' [? []]]].
+      pclearbot; destruct H11; [|inv H11].
+      pfold; apply (EG_step t2' s2'); eauto.
+      * eapply eq_sat_Ps; eauto.
+        pfold; econstructor 5; eauto.
+      * right; eapply (CIH p'); eauto.
+        -- respects; eapply sep_r; eauto.
+        -- eapply step_no_errors; eauto.
+  - revert p t1 s1 t2 s2 H H0 H1 H2 H3; pcofix CIH; intros.
+    punfold H2; red in H2; dependent induction H2.
+    + pfold; apply EG_stop.
+      * apply EG_pf in H2.
+        eapply eq_sat_Ps; eauto.
+        pfold; red; econstructor 1; eauto.
+      * intro; red in H6; destruct x0; inv H6.
+    + punfold H3; red in H3; destruct x; inv H3.
+    + destruct (stepsF_impl_stepF _ _ H6) as [?t1' [?s1' []]].
+      change (step t1 s1 t1' s1') in X.
+      pfold; apply (EG_step t1' s1'); eauto.
+      * apply EG_pf in H8.
+        eapply eq_sat_Ps; eauto.
+        pfold; econstructor 3; eauto.
+      * left; eapply H4; eauto.
+        -- respects; eapply sep_r; eauto.
+    + punfold H8; destruct H8; [| exfalso; apply H9; red; eauto ].
+      eapply H4; pclearbot; eauto.
+      -- respects; eapply sep_r; eauto.
+      -- eapply step_no_errors; eauto.
+    + punfold H8; destruct H8; [| exfalso; apply H9; red; eauto ].
+      destruct (H4 _ _ X) as [?t1' [?s1' [? []]]].
+      pclearbot; destruct H11; [|inv H11].
+      pfold; apply (EG_step t1' s1'); eauto.
+      * eapply eq_sat_Ps; eauto.
+        pfold; econstructor 5; eauto.
+      * right; eapply (CIH p'); eauto.
+        -- respects; eapply sep_r; eauto.
+        -- eapply step_no_errors; eauto.
+Qed.
+
+
+(** * Definition of our fragment of CTL **)
+
+Inductive CTLformula {S} : Type :=
+| CTL_st (P:S -> Prop)
+| CTL_and (tp1 tp2:CTLformula)
+| CTL_or (tp1 tp2:CTLformula)
+| CTL_impl (tp1 tp2:CTLformula)
+| CTL_EF (tp:CTLformula)
+| CTL_EG (tp:CTLformula)
+| CTL_AF (tp:CTLformula)
+| CTL_AG (tp:CTLformula)
+| CTL_EU (tp1 tp1:CTLformula)
+| CTL_AU (tp1 tp1:CTLformula).
+
+Fixpoint CTLsats {S R} (tp:@CTLformula S): TPred S R :=
+  match tp with
+  | CTL_st P => state_pred _ P
+  | CTL_and tp1 tp2 => (CTLsats tp1) /2\ (CTLsats tp2)
+  | CTL_or tp1 tp2 => (CTLsats tp1) \2/ (CTLsats tp2)
+  | CTL_impl tp1 tp2 => (CTLsats tp1) -2> (CTLsats tp2)
+  | CTL_EF tp => EF (CTLsats tp)
+  | CTL_EG tp => EG (CTLsats tp)
+  | CTL_AF tp => AF (CTLsats tp)
+  | CTL_AG tp => AG (CTLsats tp)
+  | CTL_EU tp1 tp2 => EU (CTLsats tp1) (CTLsats tp2)
+  | CTL_AU tp1 tp2 => AU (CTLsats tp1) (CTLsats tp2)
+  end.
+
+Inductive CTLsim {S1 S2} q: @CTLformula S1 -> @CTLformula S2 -> Prop :=
+| CTLsim_st P1 P2 : q_similar q P1 P2 -> CTLsim q (CTL_st P1) (CTL_st P2)
+| CTLsim_and tp1 tp2 tp1' tp2' : CTLsim q tp1 tp2 -> CTLsim q tp1' tp2' ->
+                                CTLsim q (CTL_and tp1 tp1') (CTL_and tp2 tp2')
+| CTLsim_or tp1 tp2 tp1' tp2' : CTLsim q tp1 tp2 -> CTLsim q tp1' tp2' ->
+                               CTLsim q (CTL_or tp1 tp1') (CTL_or tp2 tp2')
+| CTLsim_impl tp1 tp2 tp1' tp2' : CTLsim q tp1 tp2 -> CTLsim q tp1' tp2' ->
+                                 CTLsim q (CTL_impl tp1 tp1') (CTL_impl tp2 tp2')
+| CTLsim_EF tp1 tp2 : CTLsim q tp1 tp2 -> CTLsim q (CTL_EF tp1) (CTL_EF tp2)
+| CTLsim_EG tp1 tp2 : CTLsim q tp1 tp2 -> CTLsim q (CTL_EG tp1) (CTL_EG tp2)
+| CTLsim_AF tp1 tp2 : CTLsim q tp1 tp2 -> CTLsim q (CTL_AF tp1) (CTL_AF tp2)
+| CTLsim_AG tp1 tp2 : CTLsim q tp1 tp2 -> CTLsim q (CTL_AG tp1) (CTL_AG tp2)
+| CTLsim_EU tp1 tp2 tp1' tp2' : CTLsim q tp1 tp2 -> CTLsim q tp1' tp2' ->
+                               CTLsim q (CTL_EU tp1 tp1') (CTL_EU tp2 tp2')
+| CTLsim_AU tp1 tp2 tp1' tp2' : CTLsim q tp1 tp2 -> CTLsim q tp1' tp2' ->
+                               CTLsim q (CTL_AU tp1 tp1') (CTL_AU tp2 tp2')
+.
+
+Lemma tpsim_implies_eq_sat_sep_sbuter {S1 S2 R1 R2} q TP1 TP2:
+  CTLsim q TP1 TP2 -> @eq_sat_sep_sbuter S1 S2 R1 R2 q (CTLsats TP1) (CTLsats TP2).
+Proof.
+  intro tp_sim; induction tp_sim.
+  - apply eq_sat_state_preds; eauto.
+  - apply eq_sat_and; eauto.
+  - apply eq_sat_or; eauto.
+  - apply eq_sat_impl; eauto.
+  - apply eq_sat_EF; eauto.
+  - apply eq_sat_EG; eauto.
+  - apply eq_sat_AF; eauto.
+  - apply eq_sat_AG; eauto.
+  - apply eq_sat_EU; eauto.
+  - apply eq_sat_AU; eauto.
+Qed.
+
+Theorem sbuter_preserves_tpreds {S1 R1 S2 R2} p q Q t1 s1 t2 s2 TP1 TP2:
+  @sbuter S1 R1 S2 R2 p Q t1 s1 t2 s2 -> no_errors t2 s2 ->
+  CTLsim q TP1 TP2 -> pre (p ** q) (s1, s2) ->
+  CTLsats TP1 t1 s1 <-> CTLsats TP2 t2 s2.
+Proof.
+  intros sb ne tp_sim pre_pq. destruct pre_pq as [ pre_p [ pre_q sep ]].
+  eapply (tpsim_implies_eq_sat_sep_sbuter q TP1 TP2 tp_sim); eauto.
 Qed.
